platform/Depl/Depl.v
@@ -182,80 +182,6 @@ Notation "'dmodule' name ds" := (let (dts, fs) := separate ds%funcs in
 
 (** * Tactics *)
 
-(* There is a somewhat intricate little dance here to get good reduction behavior.
- * First, we normalize enough to expose potentially worrying uses of [in_dec string_dec],
- * where delta-expanding those identifiers would lead to unpleasantly large terms. *)
-Ltac depl_cbv1 := cbv beta iota zeta
-   delta [CompileModule.makeVcs CompileModule.Functions map funcOut
-         CompileModule.functionVc CompileModule.Postcondition
-         CompileModule.Formals SpecVars_ Formals_ Precondition_
-         Postcondition_ Name_ Spec_ Locals_ Body_ Logic.wellScoped
-         CompileModule.Body app CompileModule.Locals
-         CompileModule.Precondition CompileModule.SpecVars Logic.normalize
-         Statements.stmtD Statements.exprD Statements.sentail Cancel.cancel
-         Cancel.findMatchings Logic.NQuants Logic.NImpure Logic.NPure
-         Logic.nsubst Statements.lookupCon Statements.lookupCon'
-         AlgebraicDatatypes.normalizeDatatype fst snd
-         AlgebraicDatatypes.NName AlgebraicDatatypes.normalizeCon
-         AlgebraicDatatypes.Name AlgebraicDatatypes.Nonrecursive
-         AlgebraicDatatypes.Recursive AlgebraicDatatypes.Condition
-         AlgebraicDatatypes.NRecursive AlgebraicDatatypes.NNonrecursive
-         AlgebraicDatatypes.NCondition plus sumbool_rec sumbool_rect
-         Logic.notsInList Logic.notInList string_rec string_rect
-         append Ascii.ascii_dec Ascii.ascii_rec Ascii.ascii_rect
-         Bool.bool_dec bool_rec bool_rect eq_rec_r eq_rec eq_rect eq_sym
-         Statements.exprsD
-         AlgebraicDatatypes.allocatePre AlgebraicDatatypes.nsubsts
-         Peano_dec.eq_nat_dec string_eq ascii_eq Bool.eqb andb nat_rec nat_rect length
-         AlgebraicDatatypes.recursives Cancel.findMatching Logic.psubst
-         Logic.esubst Var' Cancel.sub_expr Cancel.findMatching'
-         Cancel.unify_pred Cancel.unify_expr Cancel.fos_set Cancel.unify_args Var''
-         Statements.vars_set CompileModule.vars0].
-
-(** Now we [destruct] string comparisons. *)
-Ltac streq :=
-  repeat match goal with
-           | [ |- context[string_dec ?X ?Y] ] =>
-             destruct (string_dec X Y); try congruence; [ clear ]
-           | [ |- context[in_dec string_dec ?X ?Y] ] =>
-             destruct (in_dec string_dec X Y);
-               try (exfalso; simpl in *; intuition congruence); [ clear ]
-         end.
-
-(* Next, we find the little marker predicates we used in Cancel to indicate where the
- * troubling [in_dec]s are, and we hide them inside this guy here. *)
-Definition sin_dec := in_dec string_dec.
-Ltac switch_to_sin_dec :=
-  repeat match goal with
-           | [ |- appcontext[Cancel.hide_sub ?s] ] =>
-             let s' := fresh "s'" in pose (s' := s);
-               change (in_dec string_dec) with sin_dec in s';
-                 let s'' := eval unfold s' in s' in
-                   change (Cancel.hide_sub s) with s''; clear s'
-         end.
-
-(* Finally, we can do a proper full evaluation, including unfolding of [in_dec] and [string_dec],
- * but not [sin_dec]. *)
-Ltac depl_cbv2 := cbv beta iota zeta delta [CompileModule.makeVcs CompileModule.Functions map funcOut
-  CompileModule.functionVc CompileModule.Postcondition Statements.stmtV
-  CompileModule.Formals
-  SpecVars_ Formals_ Precondition_ Postcondition_
-  Name_ Spec_ Locals_ Body_ Logic.wellScoped CompileModule.Body
-  Logic.normalize Statements.stmtD CompileModule.Precondition app
-  CompileModule.Locals Statements.sentail Statements.exprV Statements.exprD
-  Cancel.cancel Cancel.findMatchings Logic.NQuants Logic.NImpure Logic.NPure
-  Logic.nsubst CompileModule.SpecVars Cancel.findMatching Cancel.findMatching' Logic.predExt Var' Var''
-  CompileModule.vars0 Logic.exprD Statements.vars_set Logic.fo_set
-  in_dec list_rec list_rect
-  string_dec string_rec string_rect
-  Ascii.ascii_dec Ascii.ascii_rec Ascii.ascii_rect sumbool_rec sumbool_rect
-  Bool.bool_dec bool_rec bool_rect eq_rec_r eq_rec eq_rect eq_sym append
-  allocatePre nsubsts recursives
-  lookupCon lookupCon' normalizeDatatype fst snd].
-
-(* Put them all together. *)
-Ltac depl_cbv := depl_cbv1; streq; switch_to_sin_dec.
-
 Ltac isConst E :=
   match E with
     | Ascii.Ascii _ _ _ _ _ _ _ _ => idtac
@@ -275,10 +201,10 @@ Ltac depl_wf :=
           | [ H : forall x : Logic.fo_var, _ -> _ = _ |- _ ] =>
             repeat rewrite H by tauto; reflexivity
         end
-    | [ |- forall fE fE' : Logic.fo_var -> Logic.dyn, (forall x, In x _ -> fE x = fE' x) -> _ = _ ] =>
+    | [ |- forall fE fE' : Logic.fo_var -> Logic.dyn, (forall x, _ -> fE x = fE' x) -> _ = _ ] =>
       simpl; intros fE fE' Heq;
         repeat rewrite Heq by tauto; reflexivity
-    | [ |- forall x : Logic.fo_var, In x _ -> _ <> None ] => simpl In; intuition subst; congruence
+    | [ |- forall x : Logic.fo_var, _ -> _ <> None ] => simpl In; intuition subst; congruence
     | [ |- forall fE : Logic.fo_env, List.Forall _ _ ] => intro;
       repeat match goal with
                | [ |- List.Forall _ _ ] => constructor
@@ -287,9 +213,9 @@ Ltac depl_wf :=
       intros fE fE' Heq;
         repeat rewrite Heq by (simpl; congruence); reflexivity
     | [ |- In ?x ?ls ] => isConst x; isConst ls; simpl; tauto
-    | [ |- forall x : Logic.fo_var, In x _ -> exists e : Logic.expr, _ ] =>
+    | [ |- forall x : Logic.fo_var, _ -> exists e : Logic.expr, _ ] =>
       simpl; intuition (subst; simpl; eauto)
-    | [ |- forall fE fE' : Logic.fo_var -> Logic.dyn, _ -> forall e : Logic.expr, In _ _ -> _ ] =>
+    | [ |- forall fE fE' : Logic.fo_var -> Logic.dyn, _ -> forall e : Logic.expr, _ -> _ ] =>
       simpl; intuition (subst; auto)
     | [ |- forall fE1 fE2 : Logic.fo_var -> Logic.dyn,
              (forall x : Logic.fo_var, _ <> None -> fE1 x = fE2 x)
@@ -304,16 +230,20 @@ Ltac depl_wf :=
                  end; reflexivity
       end.
 
-Ltac depl := apply CompileModule.compileModule_ok; [ constructor
+Ltac depl' := apply CompileModule.compileModule_ok; [ constructor
   | hnf; NoDup
   | reflexivity
   | depl_wf
   | reflexivity
-  | depl_cbv;
-    match goal with
-      | [ |- vcs ?Ps ] => apply (vcsImp_correct Ps)
-    end;
-    repeat match goal with
-             | [ |- _ /\ _ ] => split
-           end; repeat depl_wf; unfold Logic.fo_set; simpl
+  |
   | simpl; discriminate ].
+
+Ltac dsimpl := simpl; cbv delta [Logic.fo_set Cancel.fos_set Cancel.hide_sub]; simpl.
+
+Ltac depl := depl'; dsimpl;
+             match goal with
+               | [ |- vcs ?Ps ] => apply (vcsImp_correct Ps)
+             end;
+             repeat match goal with
+                      | [ |- _ /\ _ ] => split
+                    end; repeat depl_wf.
